[ast] add mind_params_ctxt to reified declarations, adapt quoting and typing accordingly

template-coq/src/constr_quoter.ml
@@ -41,6 +41,9 @@ struct
   type quoted_mind_finiteness = Constr.t (* of type Ast.mutual_inductive_entry ?? *)
   type quoted_entry = Constr.t (* of type option (constant_entry + mutual_inductive_entry) *)
 
+  type quoted_context_decl = Constr.t (* in Ast *)
+  type quoted_context = Constr.t (* in Ast *)
+
   type quoted_one_inductive_body = Constr.t (* of type Ast.one_inductive_body *)
   type quoted_mutual_inductive_body = Constr.t (* of type Ast.mutual_inductive_body *)
   type quoted_constant_body = Constr.t (* of type Ast.constant_body *)
@@ -105,6 +108,7 @@ struct
   let sfSet = r_reify "InSet"
   let sfType = r_reify "InType"
   let tident = r_reify "ident"
+  let tname = r_reify "name"
   let tIndTy = r_reify "inductive"
   let tmkInd = r_reify "mkInd"
   let tsort_family = r_reify "sort_family"
@@ -144,6 +148,9 @@ struct
   let tConstantDecl = r_reify "ConstantDecl"
   let tInductiveDecl = r_reify "InductiveDecl"
   let tglobal_declarations = r_reify "global_declarations"
+
+  let tcontext_decl = r_reify "context_decl"
+  let tcontext = r_reify "context"
 
   let tMutual_inductive_entry = r_reify "mutual_inductive_entry"
   let tOne_inductive_entry = r_reify "one_inductive_entry"
@@ -333,6 +340,13 @@ struct
     | Sorts.InSet -> sfSet
     | Sorts.InType -> sfType
 
+  let quote_context_decl na b t =
+    pair (prod tname (Constr.mkApp (option_type, [| tTerm |]))) tTerm
+      (pair tname (Constr.mkApp (option_type, [| tTerm |])) na (quote_option tTerm b)) t
+
+  let quote_context ctx =
+    to_coq_list tcontext_decl ctx
+
   let mk_ctor_list =
     let ctor_list =
       let ctor_info_typ = prod (prod tident tTerm) tnat in
@@ -416,9 +430,9 @@ struct
     let e = mk_proj_list e in
     Constr.mkApp (tBuild_one_inductive_body, [| a; b; c; d; e |])
 
-  let mk_mutual_inductive_body p inds uctx =
+  let mk_mutual_inductive_body npars params inds uctx =
     let inds = to_coq_list tone_inductive_body inds in
-    Constr.mkApp (tBuild_mutual_inductive_body, [|p; inds; uctx|])
+    Constr.mkApp (tBuild_mutual_inductive_body, [|npars; params; inds; uctx|])
 
   let mk_constant_body ty tm uctx =
     let tm = quote_option tTerm tm in
